h2k: wip reification/compilation of the MESI case study protocol

syn/ex/Mesi/MesiDeep.v
@@ -1,3 +1,5 @@
+Require Import List.
+
 Require Import Compiler.Compiler.
 
 Require Import Hemiola.Common Hemiola.Index Hemiola.HVector.
@@ -8,225 +10,393 @@ Require Import FunctionalExtensionality.
 
 Set Implicit Arguments.
 
-Section Tests.
+(** * Utilities: move to somewhere else? *)
 
-  Lemma abcd: forall A B C D, (A <-> B) -> (C <-> D) -> (A /\ C <-> B /\ D).
-  Proof. firstorder. Qed.
+Lemma and_iff_sep: forall A B C D, (A <-> B) -> (C <-> D) -> (A /\ C <-> B /\ D).
+Proof. firstorder. Qed.
 
-  Lemma TrsMTrs_ext:
-    forall `{DecValue} `{OStateIfc} (trs1 trs2: StateMTrs),
-      (forall stm, trs1 stm = trs2 stm) ->
-      forall ost orq mins,
-        TrsMTrs trs1 ost orq mins = TrsMTrs trs2 ost orq mins.
-  Proof.
-    cbv [TrsMTrs]; intros.
-    rewrite H1; reflexivity.
-  Qed.
+Lemma TrsMTrs_ext:
+  forall `{DecValue} `{OStateIfc} (trs1 trs2: StateMTrs),
+    (forall stm, trs1 stm = trs2 stm) ->
+    forall ost orq mins,
+      TrsMTrs trs1 ost orq mins = TrsMTrs trs2 ost orq mins.
+Proof.
+  cbv [TrsMTrs]; intros.
+  rewrite H1; reflexivity.
+Qed.
 
-  Variable oidx: IdxT.
+(** * Configuration Instances *)
+Existing Instance SpecInds.NatDecValue.
+Existing Instance Mesi.ImplOStateIfc.
 
-  Instance mesiHConfig: hconfig :=
-    {| hcfg_oidx_sz := (2, 3);
-       hcfg_midx_sz := (4, 4);
-       hcfg_msg_id_sz := (3, 2);
-       hcfg_value_sz := 32;
-       hcfg_children_max_lg := 2;
+Definition HMesi := HNat 3.
+
+Instance MesiHConfig: hconfig :=
+  {| hcfg_oidx_sz := (2, 3);
+     hcfg_midx_sz := (4, 4);
+     hcfg_msg_id_sz := (3, 2);
+     hcfg_value_sz := 32;
+     hcfg_children_max_lg := 2;
+  |}.
+
+Lemma MesiHOStateIfc_host_ty_ok:
+  forall i: Fin.t ost_sz,
+    match Vector.nth [Some HValue; Some HBool; Some HMesi; None]%vector i with
+    | Some hbt => Vector.nth ost_ty i = hbtypeDenote hbt
+    | None => True
+    end.
+Proof.
+  intros.
+  refine (match i with | Fin.F1 => _ | Fin.FS _ => _ end);
+    [repeat (destruct n; [exact idProp|]);
+     destruct n; [|exact idProp];
+     reflexivity
+    |repeat (destruct n; [exact idProp|]);
+     destruct n; [|exact idProp]].
+  refine (match t with | Fin.F1 => _ | Fin.FS _ => _ end);
+    [repeat (destruct n; [exact idProp|]);
+     destruct n; [|exact idProp];
+     reflexivity
+    |repeat (destruct n; [exact idProp|]);
+     destruct n; [|exact idProp]].
+  refine (match t0 with | Fin.F1 => _ | Fin.FS _ => _ end);
+    [repeat (destruct n; [exact idProp|]);
+     destruct n; [|exact idProp];
+     reflexivity
+    |repeat (destruct n; [exact idProp|]);
+     destruct n; [|exact idProp]].
+  refine (match t1 with | Fin.F1 => _ | Fin.FS _ => _ end);
+    [repeat (destruct n; [exact idProp|]);
+     destruct n; [|exact idProp];
+     reflexivity
+    |repeat (destruct n; [exact idProp|]);
+     destruct n; [|exact idProp]].
+  apply Fin.case0; assumption.
+Defined.
+
+Instance MesiHOStateIfc: HOStateIfc :=
+  {| host_ty := [Some HValue; Some HBool; Some HMesi; None]%vector;
+     host_ty_ok := MesiHOStateIfc_host_ty_ok;
+  |}.
+
+Section DirExt.
+
+  Inductive htype_dir: Set :=
+  | HDir: htype_dir.
+
+  Definition htypeDenote_dir (ht: htype_dir): Type :=
+    match ht with
+    | HDir => Mesi.DirT
+    end.
+
+  Instance DirExtType: ExtType :=
+    {| hetype := htype_dir;
+       hetypeDenote := htypeDenote_dir
     |}.
 
-  Existing Instance SpecInds.NatDecValue.
-  Existing Instance Mesi.ImplOStateIfc.
+  Inductive hexp_dir (var: htype -> Type): htype -> Type :=
+  | HDirC: hexp_dir var (HEType HDir)
+  | HDirGet: hbexp (bvar var) HIdxO ->
+             hexp_dir var (HEType HDir) ->
+             hexp_dir var (HBType (HNat 3)).
 
-  Definition HMesi := HNat 3.
+  Fixpoint interp_hexp_dir (ost: OState) (orq: ORq Msg) (mins: list (Id Msg))
+           {ht} (he: hexp_dir htypeDenote ht): htypeDenote ht :=
+    match he in (hexp_dir _ h) return (htypeDenote h) with
+    | HDirC _ => (ost#[dir])%hvec
+    | HDirGet oidx dir => getDir (interpBExp ost oidx) (interp_hexp_dir ost orq mins dir)
+    end.
 
-  Lemma MesiHOStateIfc_host_ty_ok:
-    forall i: Fin.t ost_sz,
-      match Vector.nth [Some HValue; Some HBool; Some HMesi; None]%vector i with
-      | Some hbt => Vector.nth ost_ty i = hbtypeDenote hbt
-      | None => True
-      end.
-  Proof.
-    intros.
-    refine (match i with | Fin.F1 => _ | Fin.FS _ => _ end);
-      [repeat (destruct n; [exact idProp|]);
-       destruct n; [|exact idProp];
-       reflexivity
-      |repeat (destruct n; [exact idProp|]);
-       destruct n; [|exact idProp]].
-    refine (match t with | Fin.F1 => _ | Fin.FS _ => _ end);
-      [repeat (destruct n; [exact idProp|]);
-       destruct n; [|exact idProp];
-       reflexivity
-      |repeat (destruct n; [exact idProp|]);
-       destruct n; [|exact idProp]].
-    refine (match t0 with | Fin.F1 => _ | Fin.FS _ => _ end);
-      [repeat (destruct n; [exact idProp|]);
-       destruct n; [|exact idProp];
-       reflexivity
-      |repeat (destruct n; [exact idProp|]);
-       destruct n; [|exact idProp]].
-    refine (match t1 with | Fin.F1 => _ | Fin.FS _ => _ end);
-      [repeat (destruct n; [exact idProp|]);
-       destruct n; [|exact idProp];
-       reflexivity
-      |repeat (destruct n; [exact idProp|]);
-       destruct n; [|exact idProp]].
-    apply Fin.case0; assumption.
-  Defined.
-
-  Instance MesiHOStateIfc: HOStateIfc :=
-    {| host_ty := [Some HValue; Some HBool; Some HMesi; None]%vector;
-       host_ty_ok := MesiHOStateIfc_host_ty_ok;
+  Instance DirExtExp: ExtExp :=
+    {| heexp := hexp_dir;
+       interp_heexp := interp_hexp_dir
     |}.
 
-  Section DirExt.
+End DirExt.
 
-    Inductive htype_dir: Set :=
-    | HDir: htype_dir.
+Existing Instance DirExtType.
+Existing Instance DirExtExp.
 
-    Definition htypeDenote_dir (ht: htype_dir): Type :=
-      match ht with
-      | HDir => Mesi.DirT
-      end.
+Lemma MesiHOStateIfcFull_hostf_ty_compat:
+  forall i hbt,
+    host_ty[@i] = Some hbt ->
+    [HBType HValue; HBType HBool; HBType HMesi; HEType HDir][@i] = HBType hbt.
+Proof.
+  intros i.
+  refine (match i with | Fin.F1 => _ | Fin.FS _ => _ end);
+    [repeat (destruct n; [exact idProp|]);
+     destruct n; [|exact idProp];
+     simpl; intros; congruence
+    |repeat (destruct n; [exact idProp|]);
+     destruct n; [|exact idProp]].
+  refine (match t with | Fin.F1 => _ | Fin.FS _ => _ end);
+    [repeat (destruct n; [exact idProp|]);
+     destruct n; [|exact idProp];
+     simpl; intros; congruence
+    |repeat (destruct n; [exact idProp|]);
+     destruct n; [|exact idProp]].
+  refine (match t0 with | Fin.F1 => _ | Fin.FS _ => _ end);
+    [repeat (destruct n; [exact idProp|]);
+     destruct n; [|exact idProp];
+     simpl; intros; congruence
+    |repeat (destruct n; [exact idProp|]);
+     destruct n; [|exact idProp]].
+  refine (match t1 with | Fin.F1 => _ | Fin.FS _ => _ end);
+    [repeat (destruct n; [exact idProp|]);
+     destruct n; [|exact idProp];
+     simpl; intros; congruence
+    |repeat (destruct n; [exact idProp|]);
+     destruct n; [|exact idProp]].
+  apply Fin.case0; assumption.
+Defined.
 
-    Instance DirExtType: ExtType :=
-      {| hetype := htype_dir;
-         hetypeDenote := htypeDenote_dir
-      |}.
+Instance MesiHOStateIfcFull: HOStateIfcFull :=
+  {| hostf_ty := [HBType HValue; HBType HBool; HBType HMesi; HEType HDir];
+     hostf_ty_ok := eq_refl;
+     hostf_ty_compat := MesiHOStateIfcFull_hostf_ty_compat;
+  |}.
 
-    Inductive hexp_dir (var: htype -> Type): htype -> Type :=
-    | HDirC: hexp_dir var (HEType HDir)
-    | HDirGet: hbexp (bvar var) HIdxO ->
-               hexp_dir var (HEType HDir) ->
-               hexp_dir var (HBType (HNat 3)).
+(** * Reification *)
 
-    Fixpoint interp_hexp_dir (ost: OState) (orq: ORq Msg) (mins: list (Id Msg))
-             {ht} (he: hexp_dir htypeDenote ht): htypeDenote ht :=
-      match he in (hexp_dir _ h) return (htypeDenote h) with
-      | HDirC _ => (ost#[dir])%hvec
-      | HDirGet oidx dir => getDir (interpBExp ost oidx) (interp_hexp_dir ost orq mins dir)
-      end.
+(* Inductive OTT := One | Two | Three. *)
+(* Definition denoteOTT (n: OTT) := *)
+(*   match n with *)
+(*   | One => 1 *)
+(*   | Two => 2 *)
+(*   | Three => 3 *)
+(*   end. *)
 
-    Instance DirExtExp: ExtExp :=
-      {| heexp := hexp_dir;
-         interp_heexp := interp_hexp_dir
-      |}.
+(* Inductive FFS := Four | Five | Six. *)
+(* Definition denoteFFS (n: FFS) := *)
+(*   match n with *)
+(*   | Four => 4 *)
+(*   | Five => 5 *)
+(*   | Six => 6 *)
+(*   end. *)
 
-  End DirExt.
+(* Inductive Nat := *)
+(* | NatOTT: OTT -> Nat *)
+(* | NatFFS: FFS -> Nat *)
+(* | NatAdd: Nat -> Nat -> Nat. *)
 
-  Existing Instance DirExtType.
-  Existing Instance DirExtExp.
+(* Fixpoint denoteNat (n: Nat) := *)
+(*   match n with *)
+(*   | NatOTT no => denoteOTT no *)
+(*   | NatFFS nf => denoteFFS nf *)
+(*   | NatAdd n1 n2 => denoteNat n1 + denoteNat n2 *)
+(*   end. *)
 
-  Lemma MesiHOStateIfcFull_hostf_ty_compat:
-    forall i hbt,
-      host_ty[@i] = Some hbt ->
-      [HBType HValue; HBType HBool; HBType HMesi; HEType HDir][@i] = HBType hbt.
-  Proof.
-    intros i.
-    refine (match i with | Fin.F1 => _ | Fin.FS _ => _ end);
-      [repeat (destruct n; [exact idProp|]);
-       destruct n; [|exact idProp];
-       simpl; intros; congruence
-      |repeat (destruct n; [exact idProp|]);
-       destruct n; [|exact idProp]].
-    refine (match t with | Fin.F1 => _ | Fin.FS _ => _ end);
-      [repeat (destruct n; [exact idProp|]);
-       destruct n; [|exact idProp];
-       simpl; intros; congruence
-      |repeat (destruct n; [exact idProp|]);
-       destruct n; [|exact idProp]].
-    refine (match t0 with | Fin.F1 => _ | Fin.FS _ => _ end);
-      [repeat (destruct n; [exact idProp|]);
-       destruct n; [|exact idProp];
-       simpl; intros; congruence
-      |repeat (destruct n; [exact idProp|]);
-       destruct n; [|exact idProp]].
-    refine (match t1 with | Fin.F1 => _ | Fin.FS _ => _ end);
-      [repeat (destruct n; [exact idProp|]);
-       destruct n; [|exact idProp];
-       simpl; intros; congruence
-      |repeat (destruct n; [exact idProp|]);
-       destruct n; [|exact idProp]].
-    apply Fin.case0; assumption.
-  Defined.
+(* Goal (exists n, denoteNat n = 3 + 4). *)
+(* Proof. *)
+(*   eexists. *)
+(*   cbv [denoteNat denoteOTT denoteFFS]. *)
+(*   instantiate (1:= NatAdd _ _). *)
+(*   cbv [denoteNat denoteOTT denoteFFS]. *)
+(*   f_equal. *)
+(*   - instantiate (1:= NatOTT _). *)
+(*     cbv [denoteNat denoteOTT denoteFFS]. *)
+(*     instantiate (1:= Three). *)
+(*     reflexivity. *)
+(*   - instantiate (1:= NatFFS _). *)
+(*     cbv [denoteNat denoteOTT denoteFFS]. *)
+(*     instantiate (1:= Four). *)
+(*     reflexivity. *)
+(* Abort. *)
 
-  Instance MesiHOStateIfcFull: HOStateIfcFull :=
-    {| hostf_ty := [HBType HValue; HBType HBool; HBType HMesi; HEType HDir];
-       hostf_ty_ok := eq_refl;
-       hostf_ty_compat := MesiHOStateIfcFull_hostf_ty_compat;
-    |}.
-  
-  Definition hl1GetSImm: HRule (l1GetSImm (l1ExtOf oidx)).
-  Proof.
-    refine {| hrule_msg_from := _ |}.
+Section Deep.
+  Variable (tr: tree).
+  Hypothesis (Htr: tr <> Node nil).
 
-    - intros.
-      repeat autounfold with MesiRules.
-      cbv [immDownRule].
-      cbv [rule_precond].
+  Section L1Rules.
+    Variable oidx: IdxT.
+    
+    Definition hl1GetSImm: HRule (l1GetSImm (l1ExtOf oidx)).
+    Proof.
+      refine {| hrule_msg_from := _ |}.
 
-      apply abcd.
+      - intros; repeat autounfold with MesiRules.
+        cbv [immDownRule rule_precond].
+        apply and_iff_sep.
+        + cbv [interpMsgFrom].
+          instantiate (1:= HMsgFromExt _).
+          apply iff_refl.
 
-      + cbv [interpMsgFrom].
-        instantiate (1:= HMsgFromExt _).
-        apply iff_refl.
+        + instantiate (1:= fun var => HOPrecAnd (var:= var) _ _); simpl; apply and_iff_sep.
+          all: repeat
+                 match goal with
+                 | |- _ <-> (_ /\oprec _) _ _ _ =>
+                   instantiate (1:= HOPrecAnd _ _); simpl; apply and_iff_sep
+                 end.
 
-      + instantiate (1:= fun var => HOPrecAnd (var:= var) _ _); simpl; apply abcd.
-        all: repeat
-               match goal with
-               | |- _ <-> (_ /\oprec _) _ _ _ =>
-                 instantiate (1:= HOPrecAnd _ _); simpl; apply abcd
-               end.
+          1-4: instantiate (1:= HOPrecRqRs _ _); simpl.
+          1-4: first [instantiate (1:= HRqAccepting); apply iff_refl; fail
+                     |instantiate (1:= HRsAccepting); apply iff_refl; fail
+                     |instantiate (1:= HUpLockFree); apply iff_refl; fail
+                     |instantiate (1:= HDownLockFree); apply iff_refl; fail
+                     |instantiate (1:= HUpLockMsgId _ _); apply iff_refl; fail
+                     |instantiate (1:= HUpLockMsg); apply iff_refl; fail
+                     |instantiate (1:= HUpLockIdxBack); apply iff_refl; fail
+                     |instantiate (1:= HUpLockBackNone); apply iff_refl; fail
+                     |instantiate (1:= HDownLockMsgId _ _); apply iff_refl; fail
+                     |instantiate (1:= HDownLockMsg); apply iff_refl; fail
+                     |instantiate (1:= HDownLockIdxBack); apply iff_refl; fail
+                     |instantiate (1:= HMsgIdFrom _); apply iff_refl; fail].
 
-        1-4: instantiate (1:= HOPrecRqRs _ _); simpl.
-        1-4: first [instantiate (1:= HRqAccepting); apply iff_refl; fail
-                   |instantiate (1:= HRsAccepting); apply iff_refl; fail
-                   |instantiate (1:= HUpLockFree); apply iff_refl; fail
-                   |instantiate (1:= HDownLockFree); apply iff_refl; fail
-                   |instantiate (1:= HUpLockMsgId _ _); apply iff_refl; fail
-                   |instantiate (1:= HUpLockMsg); apply iff_refl; fail
-                   |instantiate (1:= HUpLockIdxBack); apply iff_refl; fail
-                   |instantiate (1:= HUpLockBackNone); apply iff_refl; fail
-                   |instantiate (1:= HDownLockMsgId _ _); apply iff_refl; fail
-                   |instantiate (1:= HDownLockMsg); apply iff_refl; fail
-                   |instantiate (1:= HDownLockIdxBack); apply iff_refl; fail
-                   |instantiate (1:= HMsgIdFrom _); apply iff_refl; fail].
+          instantiate (1:= HOPrecProp _); simpl.
+          instantiate (1:= HNatLe (w:= 3) _ _); simpl.
+          instantiate (2:= HBExp (HBConst _ (HBConstNat _ Mesi.mesiS))); simpl.
+          instantiate (1:= HBExp (HOstVal _ status eq_refl)); simpl.
+          apply iff_refl.
 
-        instantiate (1:= HOPrecProp _); simpl.
-        instantiate (1:= HNatLe (w:= 3) _ _); simpl.
-        instantiate (2:= HBExp (HBConst _ (HBConstNat _ Mesi.mesiS))); simpl.
-        instantiate (1:= HBExp (HOstVal _ status eq_refl)); simpl.
-        setoid_rewrite <-eq_rect_eq.
-        apply iff_refl.
+      - intros.
+        repeat autounfold with MesiRules.
+        cbv [immDownRule rule_trs].
 
-    - intros.
-      repeat autounfold with MesiRules.
-      cbv [immDownRule].
-      cbv [rule_trs].
-
-      instantiate (1:= HTrsMTrs (HMTrs _)); simpl.
-      apply TrsMTrs_ext; intros.
-      instantiate (1:= fun var => HBind (var:= var) _ _); simpl.
-      instantiate (3:= HGetFirstMsg); simpl.
-      instantiate (1:= fun msg => HRet _ _ _).
-      simpl; repeat f_equal.
-      apply functional_extensionality; intros msg.
-      repeat f_equal.
-      { instantiate (1:= HOStateI _); reflexivity. }
-      { instantiate (1:= HORqI _); reflexivity. }
-      { instantiate (1:= HMsgOutExt _ _).
+        instantiate (1:= HTrsMTrs (HMTrs _)); simpl.
+        apply TrsMTrs_ext; intros.
+        instantiate (1:= fun var => HBind (var:= var) _ _); simpl.
+        instantiate (3:= HGetFirstMsg); simpl.
+        instantiate (1:= fun msg => HRet _ _ _).
         simpl; repeat f_equal.
-        { cbv [rsMsg miv_id miv_value].
-          instantiate (1:= HBExp (HMsgB _ _ _)).
-          simpl; f_equal.
-          { instantiate (1:= HBConst _ (HBConstIdx hcfg_msg_id_sz _)); reflexivity. }
-          { instantiate (1:= HBConst _ (HBConstBool _)); reflexivity. }
-          { instantiate (1:= HOstVal _ val eq_refl).
-            simpl; setoid_rewrite <-eq_rect_eq.
-            reflexivity.
+        apply functional_extensionality; intros msg.
+        repeat f_equal.
+        { instantiate (1:= HOStateI _); reflexivity. }
+        { instantiate (1:= HORqI _); reflexivity. }
+        { instantiate (1:= HMsgOutExt _ _).
+          simpl; repeat f_equal.
+          { cbv [rsMsg miv_id miv_value].
+            instantiate (1:= HBExp (HMsgB _ _ _)).
+            simpl; f_equal.
+            { instantiate (1:= HBConst _ (HBConstIdx hcfg_msg_id_sz _)); reflexivity. }
+            { instantiate (1:= HBConst _ (HBConstBool _)); reflexivity. }
+            { instantiate (1:= HOstVal _ val eq_refl).
+              reflexivity.
+            }
           }
         }
-      }
+    Defined.
+
+    Definition hl1GetSRqUpUp: HRule (l1GetSRqUpUp oidx (l1ExtOf oidx)).
+    Proof.
+      refine {| hrule_msg_from := _ |}.
+
+      - intros; repeat autounfold with MesiRules.
+        cbv [rqUpUpRule rule_precond].
+        apply and_iff_sep.
+        + cbv [interpMsgFrom].
+          instantiate (1:= HMsgFromExt _).
+          apply iff_refl.
+
+        + instantiate (1:= fun var => HOPrecAnd (var:= var) _ _); simpl; apply and_iff_sep.
+          all: repeat
+                 match goal with
+                 | |- _ <-> (_ /\oprec _) _ _ _ =>
+                   instantiate (1:= HOPrecAnd _ _); simpl; apply and_iff_sep
+                 end.
+
+          1-3: instantiate (1:= HOPrecRqRs _ _); simpl.
+          1-3: first [instantiate (1:= HRqAccepting); apply iff_refl; fail
+                     |instantiate (1:= HRsAccepting); apply iff_refl; fail
+                     |instantiate (1:= HUpLockFree); apply iff_refl; fail
+                     |instantiate (1:= HDownLockFree); apply iff_refl; fail
+                     |instantiate (1:= HUpLockMsgId _ _); apply iff_refl; fail
+                     |instantiate (1:= HUpLockMsg); apply iff_refl; fail
+                     |instantiate (1:= HUpLockIdxBack); apply iff_refl; fail
+                     |instantiate (1:= HUpLockBackNone); apply iff_refl; fail
+                     |instantiate (1:= HDownLockMsgId _ _); apply iff_refl; fail
+                     |instantiate (1:= HDownLockMsg); apply iff_refl; fail
+                     |instantiate (1:= HDownLockIdxBack); apply iff_refl; fail
+                     |instantiate (1:= HMsgIdFrom _); apply iff_refl; fail].
+
+          instantiate (1:= HOPrecProp _); simpl.
+          instantiate (1:= HNatLe (w:= 3) _ _); simpl.
+          instantiate (1:= HBExp (HBConst _ (HBConstNat _ Mesi.mesiI))); simpl.
+          instantiate (1:= HBExp (HOstVal _ status eq_refl)); simpl.
+          apply iff_refl.
+
+      - intros.
+        repeat autounfold with MesiRules.
+        cbv [rqUpUpRule rule_trs].
+
+        instantiate (1:= HTrsMTrs (HMTrs _)); simpl.
+        apply TrsMTrs_ext; intros.
+        instantiate (1:= fun var => HBind (var:= var) _ _); simpl.
+        instantiate (3:= HGetFirstMsg); simpl.
+        instantiate (1:= fun msg => HRet _ _ _).
+        simpl; repeat f_equal.
+        apply functional_extensionality; intros msg.
+        repeat f_equal.
+        { instantiate (1:= HOStateI _); reflexivity. }
+        { instantiate (1:= HUpdUpLock _ _ _).
+          simpl; f_equal.
+          { instantiate (1:= HBExp (HVar _ _ _)).
+            simpl; reflexivity.
+          }
+          { instantiate (1:= HBExp (HBConst _ (HBConstIdx hcfg_midx_sz _))).
+            simpl; reflexivity.
+          }
+          { instantiate (1:= HBExp (HBConst _ (HBConstIdx hcfg_midx_sz _))).
+            simpl; reflexivity.
+          }
+        }
+        { instantiate (1:= HMsgOutUp _ _).
+          simpl; repeat f_equal.
+          instantiate (1:= HBExp (HMsgB _ _ _)).
+          cbv [rqMsg]; simpl; f_equal.
+          { instantiate (1:= HBConst _ (HBConstIdx hcfg_msg_id_sz _)).
+            simpl; reflexivity.
+          }
+          { instantiate (1:= HBConst _ (HBConstBool _)).
+            simpl; reflexivity.
+          }
+          { apply TODO. (* HValue constant (inst. NatDecValue) *)
+          }
+        }
+    Abort.
+
+  End L1Rules.
+    
+  Section Object.
+    Variable (oidx: IdxT).
+
+    Definition hl1: HObject (Mesi.l1 oidx).
+    Proof.
+      refine {| hobj_rules_ok := _ |}.
+      cbv [l1 obj_rules].
+      repeat match goal with
+             | |- map _ _ = (_ :: _)%list => instantiate (1:= (_ :: _)%list); simpl; f_equal
+             | |- map _ _ = nil => instantiate (1:= nil); reflexivity
+             end.
+      all: instantiate (1:= existT _ _ _); reflexivity.
+
+      Unshelve. all: cbv beta.
+      1: exact (hl1GetSImm _).
+      all: apply TODO.
+    Defined.
+    
+    Definition hli: HObject (Mesi.li tr oidx) := TODO _.
+    Definition hmem: HObject (Mesi.mem tr oidx) := TODO _.
+
+  End Object.
+  
+  Definition himpl: HSystem (Mesi.impl Htr).
+  Proof.
+    refine {| hsys_objs_ok := _ |}.
+    cbv [impl sys_objs].
+    instantiate (1:= (_ ++ _)%list); rewrite map_app; f_equal.
+
+    - instantiate (1:= (_ :: _)%list); simpl; f_equal.
+      + instantiate (1:= existT _ _ (hmem _)); reflexivity.
+      + instantiate (1:= map (fun i => existT _ _ (hli i))
+                             (tl (c_li_indices (snd (tree2Topo tr 0))))).
+        rewrite map_map.
+        reflexivity.
+
+    - instantiate (1:= map (fun i => existT _ _ (hl1 i))
+                           (c_l1_indices (snd (tree2Topo tr 0)))).
+      rewrite map_map.
+      reflexivity.
   Defined.
 
-End Tests.
+End Deep.
 
